src/Promising.v
@@ -692,6 +692,14 @@ Module Machine.
   .
   Hint Constructors no_promise.
 
+  Lemma is_terminal_no_promise
+        m
+        (TERMINAL: is_terminal m):
+    no_promise m.
+  Proof.
+    econs. i. eapply TERMINAL. eauto.
+  Qed.
+
   Inductive step0 (eustep: forall (tid:Id.t) (eu1 eu2:ExecUnit.t), Prop) (m1 m2:t): Prop :=
   | step0_intro
       tid st1 lc1 st2 lc2
@@ -716,12 +724,6 @@ Module Machine.
       (CONSISTENT: consistent eustep m2)
   .
   Hint Constructors step.
-
-  Inductive pf_init (p:program) (m:t): Prop :=
-  | init_pf_intro
-      (STEP: rtc (step0 ExecUnit.promise_step) (init p) m)
-      (CONSISTENT: consistent ExecUnit.state_step m)
-  .
 
   Lemma no_promise_consistent
         eustep m
@@ -846,15 +848,6 @@ Module Machine.
     - eapply step0_promise_step_wf; eauto.
   Qed.
 
-  Lemma pf_init_wf p m
-        (INIT: pf_init p m):
-    wf m.
-  Proof.
-    inv INIT. clear CONSISTENT.
-    generalize (init_wf p). induction STEP; ss.
-    i. apply IHSTEP. eapply step0_promise_step_wf; eauto.
-  Qed.
-
   Lemma step0_mon
         (eustep1 eustep2: _ -> _ -> _ -> Prop)
         (EUSTEP: forall tid m1 m2, eustep1 tid m1 m2 -> eustep2 tid m1 m2):
@@ -880,185 +873,12 @@ Module Machine.
     revert CONSISTENT. induction STEP; ss.
     i. apply IHSTEP. apply H.
   Qed.
+
+  Inductive pf_exec (p:program) (m:t): Prop :=
+  | pf_exec_intro
+      m1
+      (STEP1: rtc (step0 ExecUnit.promise_step) (init p) m1)
+      (STEP2: rtc (step0 ExecUnit.state_step) m1 m)
+      (NOPROMISE: no_promise m)
+  .
 End Machine.
-
-Lemma reorder_state_step_promise_step
-      m1 m2 m3
-      (WF: Machine.wf m1)
-      (STEP1: Machine.step0 ExecUnit.state_step m1 m2)
-      (STEP2: Machine.step0 ExecUnit.promise_step m2 m3):
-  exists m2',
-    <<STEP: Machine.step0 ExecUnit.promise_step m1 m2'>> /\
-    <<STEP: Machine.step0 ExecUnit.state_step m2' m3>>.
-Proof.
-  destruct m1 as [tpool1 mem1].
-  destruct m2 as [tpool2 mem2].
-  destruct m3 as [tpool3 mem3].
-  inv STEP1. inv STEP2. ss. subst.
-  revert FIND0. rewrite IdMap.add_spec. condtac.
-  - (* same thread *)
-    inversion e. i. inv FIND0.
-    inv STEP. inv STEP0. inv LOCAL0. inv MEM2. ss. subst.
-    eexists (Machine.mk _ _). esplits.
-    + econs; eauto; ss. econs; ss. econs; ss.
-    + econs; ss.
-      * rewrite IdMap.add_spec. instantiate (3 := tid). condtac; [|congr]. eauto.
-      * econs; eauto; ss.
-        instantiate (1 :=
-                       Local.mk
-                         lc0.(Local.coh)
-                         lc0.(Local.vrp)
-                         lc0.(Local.vwp)
-                         lc0.(Local.vrm)
-                         lc0.(Local.vwm)
-                         lc0.(Local.vcap)
-                         lc0.(Local.vrel)
-                         lc0.(Local.fwdbank)
-                         lc0.(Local.exbank)
-                         (Promises.set (S (length mem1)) lc0.(Local.promises))).
-        inv LOCAL.
-        { econs 1; eauto. inv LC. econs; ss. }
-        { econs 2; eauto. inv STEP. ss.
-          exploit ExecUnit.read_wf; try exact MSG. i.
-          econs; eauto; ss.
-          - ii. eapply LATEST; eauto.
-            rewrite nth_error_app1 in MSG0; ss.
-            eapply lt_le_trans; eauto.
-            inv WF. exploit WF0; eauto. i. inv x. ss. inv LOCAL.
-            repeat apply join_spec; ExecUnit.tac.
-            inv STATE. apply ExecUnit.expr_wf. ss.
-          - apply Memory.read_mon. ss.
-        }
-        { econs 3; eauto. inv STEP. ss.
-          exploit ExecUnit.get_msg_wf; try exact MSG. i.
-          econs; eauto; ss.
-          - i. exploit EX; eauto. i. des.
-            esplits; eauto. ii.
-            rewrite nth_error_app1 in MSG0; [|lia].
-            eapply LATEST; eauto.
-            rewrite <- READ. unfold Memory.read. destruct tsx; ss.
-            rewrite nth_error_app1; [|lia]. ss.
-          - rewrite <- MSG. unfold Memory.get_msg. destruct ts; ss.
-            rewrite nth_error_app1; [|lia]. ss.
-          - f_equal. apply Promises.set_unset.
-            ii. subst. lia.
-        }
-        { econs 4; eauto. inv STEP. econs; eauto. }
-        { econs 5; eauto. inv STEP. econs; eauto. }
-        { econs 6; eauto. inv STEP. econs; eauto. }
-        { econs 7; eauto. inv STEP. econs; eauto. }
-        { econs 8; eauto. inv STEP. econs; eauto. }
-      * rewrite ? IdMap.add_add. eauto.
-  - (* diff thread *)
-    inv STEP. inv STEP0. inv LOCAL0. inv MEM2. ss. subst.
-    eexists (Machine.mk _ _). esplits.
-    + econs; eauto; ss. econs; ss. econs; ss.
-    + econs; ss.
-      * rewrite IdMap.add_spec. instantiate (3 := tid). condtac; [|by eauto].
-        inversion e0. subst. congr.
-      * econs; eauto; ss.
-        inv LOCAL.
-        { econs 1; eauto. }
-        { econs 2; eauto. inv STEP. econs; eauto.
-          - ii. eapply LATEST; eauto.
-            destruct (lt_dec ts0 (length mem1)).
-            { rewrite nth_error_app1 in MSG0; ss. }
-            contradict n.
-            eapply View.lt_le_trans; [apply TS2|].
-            inv WF. exploit WF0; try exact FIND; eauto. i. inv x. inv LOCAL. ss.
-            repeat apply join_spec; ExecUnit.tac.
-            inv STATE. apply ExecUnit.expr_wf. ss.
-          - apply Memory.read_mon. ss.
-        }
-        { econs 3; eauto. inv STEP. econs; eauto.
-          - i. exploit EX; eauto. i. des. esplits; eauto.
-            exploit ExecUnit.get_msg_wf; eauto. i.
-            ii. des. rewrite nth_error_app1 in MSG0; [|lia].
-            eapply LATEST; eauto.
-            rewrite <- READ. unfold Memory.read. destruct tsx; ss.
-            rewrite nth_error_app1; ss. lia.
-          - apply Memory.get_msg_mon. ss.
-        }
-        { econs 4; eauto. }
-        { econs 5; eauto. }
-        { econs 6; eauto. }
-        { econs 7; eauto. }
-        { econs 8; eauto. }
-      * apply IdMap.add_add_diff. ss.
-Qed.
-
-Lemma reorder_state_step_rtc_promise_step
-      m1 m2 m3
-      (WF: Machine.wf m1)
-      (STEP1: Machine.step0 ExecUnit.state_step m1 m2)
-      (STEP2: rtc (Machine.step0 ExecUnit.promise_step) m2 m3):
-  exists m2',
-    <<STEP: rtc (Machine.step0 ExecUnit.promise_step) m1 m2'>> /\
-    <<STEP: Machine.step0 ExecUnit.state_step m2' m3>>.
-Proof.
-  revert m1 WF STEP1. induction STEP2; eauto.
-  i. exploit reorder_state_step_promise_step; eauto. i. des.
-  exploit Machine.step0_promise_step_wf; eauto. i.
-  exploit IHSTEP2; eauto. i. des.
-  esplits; cycle 1; eauto.
-Qed.
-
-Lemma split_rtc_step0
-      m1 m3
-      (WF: Machine.wf m1)
-      (STEP: rtc (Machine.step0 ExecUnit.step) m1 m3):
-  exists m2,
-    <<STEP: rtc (Machine.step0 ExecUnit.promise_step) m1 m2>> /\
-    <<STEP: rtc (Machine.step0 ExecUnit.state_step) m2 m3>>.
-Proof.
-  revert WF. induction STEP; eauto. i.
-  exploit Machine.step0_step_wf; eauto. i.
-  exploit IHSTEP; eauto. i. des.
-  inv H. inv STEP2.
-  - exploit reorder_state_step_rtc_promise_step; try exact WF; eauto. i. des.
-    esplits; eauto.
-  - esplits; cycle 1; eauto.
-Qed.
-
-Theorem promising_to_pf_promising
-        p m
-        (STEP: rtc (Machine.step ExecUnit.step) (Machine.init p) m)
-        (NOPROMISE: Machine.no_promise m):
-  exists m',
-    <<INIT: Machine.pf_init p m'>> /\
-    <<STEP: rtc (Machine.step ExecUnit.state_step) m' m>>.
-Proof.
-  generalize (Machine.init_wf p). intro WF.
-  generalize (Machine.init_consistent ExecUnit.step p). intro CONSISTENT.
-  exploit Machine.rtc_step_consistent; eauto. i.
-  exploit rtc_mon.
-  { instantiate (1 := Machine.step0 ExecUnit.step).
-    instantiate (1 := Machine.step ExecUnit.step).
-    i. inv H. ss.
-  }
-  { eauto. }
-  i. exploit split_rtc_step0; eauto. i. des.
-  esplits.
-  - econs; eauto.
-  - apply Machine.rtc_step0_step; ss. econs; eauto.
-Qed.
-
-Theorem pf_promising_to_promising
-        p m1 m2
-        (INIT: Machine.pf_init p m1)
-        (STEP: rtc (Machine.step ExecUnit.state_step) m1 m2)
-        (NOPROMISE: Machine.no_promise m2):
-  rtc (Machine.step ExecUnit.step) (Machine.init p) m2.
-Proof.
-  inv INIT.
-  exploit Machine.rtc_step_consistent; try exact STEP; eauto. i.
-  apply Machine.rtc_step0_step; cycle 1.
-  { econs; eauto. }
-  etrans.
-  - eapply rtc_mon; cycle 1; eauto.
-    i. eapply Machine.step0_mon; cycle 1; eauto.
-    econs 2; eauto.
-  - eapply rtc_mon; cycle 1; eauto.
-    i. inv H. exploit Machine.step0_mon; cycle 1; eauto.
-    econs 1; eauto.
-Qed.
