src/Reorder.v
@@ -1,0 +1,195 @@
+Require Import Relations.
+Require Import EquivDec.
+Require Import Equality.
+Require Import List.
+Require Import Bool.
+Require Import Lia.
+Require Import NArith.
+Require Import PArith.
+Require Import ZArith.
+Require Import FMapPositive.
+Require Import FSetPositive.
+Require Import EquivDec.
+Require Import sflib.
+
+Require Import Basic.
+Require Import Order.
+Require Import Time.
+Require Import Lang.
+Require Import Promising.
+
+Set Implicit Arguments.
+
+
+Lemma reorder_state_step_promise_step
+      m1 m2 m3
+      (WF: Machine.wf m1)
+      (STEP1: Machine.step0 ExecUnit.state_step m1 m2)
+      (STEP2: Machine.step0 ExecUnit.promise_step m2 m3):
+  exists m2',
+    <<STEP: Machine.step0 ExecUnit.promise_step m1 m2'>> /\
+    <<STEP: Machine.step0 ExecUnit.state_step m2' m3>>.
+Proof.
+  destruct m1 as [tpool1 mem1].
+  destruct m2 as [tpool2 mem2].
+  destruct m3 as [tpool3 mem3].
+  inv STEP1. inv STEP2. ss. subst.
+  revert FIND0. rewrite IdMap.add_spec. condtac.
+  - (* same thread *)
+    inversion e. i. inv FIND0.
+    inv STEP. inv STEP0. inv LOCAL0. inv MEM2. ss. subst.
+    eexists (Machine.mk _ _). esplits.
+    + econs; eauto; ss. econs; ss. econs; ss.
+    + econs; ss.
+      * rewrite IdMap.add_spec. instantiate (3 := tid). condtac; [|congr]. eauto.
+      * econs; eauto; ss.
+        instantiate (1 :=
+                       Local.mk
+                         lc0.(Local.coh)
+                         lc0.(Local.vrp)
+                         lc0.(Local.vwp)
+                         lc0.(Local.vrm)
+                         lc0.(Local.vwm)
+                         lc0.(Local.vcap)
+                         lc0.(Local.vrel)
+                         lc0.(Local.fwdbank)
+                         lc0.(Local.exbank)
+                         (Promises.set (S (length mem1)) lc0.(Local.promises))).
+        inv LOCAL.
+        { econs 1; eauto. inv LC. econs; ss. }
+        { econs 2; eauto. inv STEP. ss.
+          exploit ExecUnit.read_wf; try exact MSG. i.
+          econs; eauto; ss.
+          - ii. eapply LATEST; eauto.
+            rewrite nth_error_app1 in MSG0; ss.
+            eapply lt_le_trans; eauto.
+            inv WF. exploit WF0; eauto. i. inv x. ss. inv LOCAL.
+            repeat apply join_spec; ExecUnit.tac.
+            inv STATE. apply ExecUnit.expr_wf. ss.
+          - apply Memory.read_mon. ss.
+        }
+        { econs 3; eauto. inv STEP. ss.
+          exploit ExecUnit.get_msg_wf; try exact MSG. i.
+          econs; eauto; ss.
+          - i. exploit EX; eauto. i. des.
+            esplits; eauto. ii.
+            rewrite nth_error_app1 in MSG0; [|lia].
+            eapply LATEST; eauto.
+            rewrite <- READ. unfold Memory.read. destruct tsx; ss.
+            rewrite nth_error_app1; [|lia]. ss.
+          - rewrite <- MSG. unfold Memory.get_msg. destruct ts; ss.
+            rewrite nth_error_app1; [|lia]. ss.
+          - f_equal. apply Promises.set_unset.
+            ii. subst. lia.
+        }
+        { econs 4; eauto. inv STEP. econs; eauto. }
+        { econs 5; eauto. inv STEP. econs; eauto. }
+        { econs 6; eauto. inv STEP. econs; eauto. }
+        { econs 7; eauto. inv STEP. econs; eauto. }
+        { econs 8; eauto. inv STEP. econs; eauto. }
+      * rewrite ? IdMap.add_add. eauto.
+  - (* diff thread *)
+    inv STEP. inv STEP0. inv LOCAL0. inv MEM2. ss. subst.
+    eexists (Machine.mk _ _). esplits.
+    + econs; eauto; ss. econs; ss. econs; ss.
+    + econs; ss.
+      * rewrite IdMap.add_spec. instantiate (3 := tid). condtac; [|by eauto].
+        inversion e0. subst. congr.
+      * econs; eauto; ss.
+        inv LOCAL.
+        { econs 1; eauto. }
+        { econs 2; eauto. inv STEP. econs; eauto.
+          - ii. eapply LATEST; eauto.
+            destruct (lt_dec ts0 (length mem1)).
+            { rewrite nth_error_app1 in MSG0; ss. }
+            contradict n.
+            eapply View.lt_le_trans; [apply TS2|].
+            inv WF. exploit WF0; try exact FIND; eauto. i. inv x. inv LOCAL. ss.
+            repeat apply join_spec; ExecUnit.tac.
+            inv STATE. apply ExecUnit.expr_wf. ss.
+          - apply Memory.read_mon. ss.
+        }
+        { econs 3; eauto. inv STEP. econs; eauto.
+          - i. exploit EX; eauto. i. des. esplits; eauto.
+            exploit ExecUnit.get_msg_wf; eauto. i.
+            ii. des. rewrite nth_error_app1 in MSG0; [|lia].
+            eapply LATEST; eauto.
+            rewrite <- READ. unfold Memory.read. destruct tsx; ss.
+            rewrite nth_error_app1; ss. lia.
+          - apply Memory.get_msg_mon. ss.
+        }
+        { econs 4; eauto. }
+        { econs 5; eauto. }
+        { econs 6; eauto. }
+        { econs 7; eauto. }
+        { econs 8; eauto. }
+      * apply IdMap.add_add_diff. ss.
+Qed.
+
+Lemma reorder_state_step_rtc_promise_step
+      m1 m2 m3
+      (WF: Machine.wf m1)
+      (STEP1: Machine.step0 ExecUnit.state_step m1 m2)
+      (STEP2: rtc (Machine.step0 ExecUnit.promise_step) m2 m3):
+  exists m2',
+    <<STEP: rtc (Machine.step0 ExecUnit.promise_step) m1 m2'>> /\
+    <<STEP: Machine.step0 ExecUnit.state_step m2' m3>>.
+Proof.
+  revert m1 WF STEP1. induction STEP2; eauto.
+  i. exploit reorder_state_step_promise_step; eauto. i. des.
+  exploit Machine.step0_promise_step_wf; eauto. i.
+  exploit IHSTEP2; eauto. i. des.
+  esplits; cycle 1; eauto.
+Qed.
+
+Lemma split_rtc_step0
+      m1 m3
+      (WF: Machine.wf m1)
+      (STEP: rtc (Machine.step0 ExecUnit.step) m1 m3):
+  exists m2,
+    <<STEP: rtc (Machine.step0 ExecUnit.promise_step) m1 m2>> /\
+    <<STEP: rtc (Machine.step0 ExecUnit.state_step) m2 m3>>.
+Proof.
+  revert WF. induction STEP; eauto. i.
+  exploit Machine.step0_step_wf; eauto. i.
+  exploit IHSTEP; eauto. i. des.
+  inv H. inv STEP2.
+  - exploit reorder_state_step_rtc_promise_step; try exact WF; eauto. i. des.
+    esplits; eauto.
+  - esplits; cycle 1; eauto.
+Qed.
+
+Theorem promising_to_pf_promising
+        p m
+        (STEP: rtc (Machine.step ExecUnit.step) (Machine.init p) m)
+        (NOPROMISE: Machine.no_promise m):
+  Machine.pf_exec p m.
+Proof.
+  generalize (Machine.init_wf p). intro WF.
+  generalize (Machine.init_consistent ExecUnit.step p). intro CONSISTENT.
+  exploit Machine.rtc_step_consistent; eauto. i.
+  exploit rtc_mon.
+  { instantiate (1 := Machine.step0 ExecUnit.step).
+    instantiate (1 := Machine.step ExecUnit.step).
+    i. inv H. ss.
+  }
+  { eauto. }
+  i. exploit split_rtc_step0; eauto. i. des.
+  econs; eauto.
+Qed.
+
+Theorem pf_promising_to_promising
+        p m
+        (EXEC: Machine.pf_exec p m):
+  <<STEP: rtc (Machine.step ExecUnit.step) (Machine.init p) m>> /\
+  <<NOPROMISE: Machine.no_promise m>>.
+Proof.
+  inv EXEC. esplits; ss.
+  apply Machine.rtc_step0_step; cycle 1.
+  { apply Machine.no_promise_consistent. ss. }
+  etrans.
+  - eapply rtc_mon; cycle 1; eauto.
+    apply Machine.step0_mon. right. ss.
+  - eapply rtc_mon; cycle 1; eauto.
+    apply Machine.step0_mon. left. ss.
+Qed.
